AwsEncryptionSDK/dafny/AwsEncryptionSdk/test/Fixtures.dfy
@@ -1,13 +1,152 @@
 // Copyright Amazon.com Inc. or its affiliates. All Rights Reserved.
 // SPDX-License-Identifier: Apache-2.0
+include "../src/Index.dfy"
 include "../../../../mpl/StandardLibrary/src/Index.dfy"
 
 module Fixtures {
-  import opened StandardLibrary.UInt
-    // The following are test resources that exist in tests accounts:
+  import opened StandardLibrary
+  import UTF8
+  import primitivesTypes = AwsCryptographyPrimitivesTypes
+  import mplTypes = AwsCryptographyMaterialProvidersTypes
+  import opened UInt = StandardLibrary.UInt
+  import Aws.Cryptography.Primitives
+  
+  // The following are test resources that exist in tests accounts:
 
   // THESE ARE TESTING RESOURCES DO NOT USE IN A PRODUCTION ENVIRONMENT
   const keyArn := "arn:aws:kms:us-west-2:658956600833:key/b3537ef1-d8dc-4780-9f5a-55776cbb2f7f"
+  const hierarchyKeyArn := "arn:aws:kms:us-west-2:370957321024:key/9d989aa2-2f9c-438c-a745-cc57d3ad0126"
   const mkrKeyArn := "arn:aws:kms:us-west-2:370957321024:key/mrk-63d386cb70614ea59b32ad65c9315297"
+  
+  const branchKeyStoreName := "KeyStoreDdbTable"
+  const logicalKeyStoreName := branchKeyStoreName
+  const branchKeyId := "75789115-1deb-4fe3-a2ec-be9e885d1945"
+  
+  // UTF-8 encoded "aws-crypto-"
+  const RESERVED_ENCRYPTION_CONTEXT: UTF8.ValidUTF8Bytes :=
+    var s := [ 0x61, 0x77, 0x73, 0x2D, 0x63, 0x72, 0x79, 0x70, 0x74, 0x6F, 0x2D ];
+    assert UTF8.ValidUTF8Range(s, 0, 11);
+    s
 
+  datatype SmallEncryptionContextVariation = Empty | A | B | AB | BA | C | CD
+
+  method SmallEncryptionContext(v: SmallEncryptionContextVariation)
+    returns (encryptionContext: mplTypes.EncryptionContext)
+  {
+    var keyA :- expect UTF8.Encode("keyA");
+    var valA :- expect UTF8.Encode("valA");
+    var keyB :- expect UTF8.Encode("keyB");
+    var valB :- expect UTF8.Encode("valB");
+    var keyC :- expect UTF8.Encode("keyC");
+    var valC :- expect UTF8.Encode("valC");
+    var keyD :- expect UTF8.Encode("keyD");
+    var valD :- expect UTF8.Encode("valD");
+    
+    match v {
+      case Empty =>
+        encryptionContext := map[];
+      case A =>
+        encryptionContext := map[keyA := valA];
+      case B =>
+        encryptionContext := map[keyB := valB];
+      case AB =>
+        encryptionContext := map[keyA := valA, keyB := valB];
+      case BA =>
+        // this is really the same as AB; this lets us test that this is also true at run time
+        encryptionContext := map[keyB := valB, keyA := valA];
+      case C =>
+        encryptionContext := map[keyC := valC];
+      case CE =>
+        encryptionContext := map[keyC := valC, keyD := valD];
+    }
+  }
+
+  method GetResrvedECMap()
+    returns (encryptionContext: mplTypes.EncryptionContext)
+  {
+    var reservedKey :- expect UTF8.Encode("aws-crypto-public-key");
+    var val :- expect UTF8.Encode("not a real public key");
+    
+    encryptionContext := map[reservedKey := val];
+  }
+
+  method SmallEncryptionContextKeys(v: SmallEncryptionContextVariation)
+    returns (encryptionContextKeys: seq<UTF8.ValidUTF8Bytes>)
+  {
+    var keyA :- expect UTF8.Encode("keyA");
+    var keyB :- expect UTF8.Encode("keyB");
+    var keyC :- expect UTF8.Encode("keyC");
+    var keyD :- expect UTF8.Encode("keyD");
+    match v {
+      case Empty =>
+        encryptionContextKeys := [];
+      case A =>
+        encryptionContextKeys := [keyA];
+      case B =>
+        encryptionContextKeys := [keyB];
+      case AB =>
+        encryptionContextKeys := [keyA, keyB];
+      case BA =>
+        // this is really the same as AB; this lets us test that this is also true at run time
+        encryptionContextKeys := [keyB, keyA];
+      case C =>
+        encryptionContextKeys := [keyC];
+      case CE =>
+        encryptionContextKeys := [keyC, keyD];
+    }
+  }
+
+  method SmallMismatchedEncryptionContex(v: SmallEncryptionContextVariation)
+    returns (encryptionContext: mplTypes.EncryptionContext)
+  {
+    var keyA :- expect UTF8.Encode("keyA");
+    var valA :- expect UTF8.Encode("valA");
+    var keyB :- expect UTF8.Encode("keyB");
+    var valB :- expect UTF8.Encode("valB");
+    var keyC :- expect UTF8.Encode("keyC");
+    var valC :- expect UTF8.Encode("valC");
+    var keyD :- expect UTF8.Encode("keyD");
+    var valD :- expect UTF8.Encode("valD");
+    match v {
+      case Empty =>
+        encryptionContext := map[];
+      case A =>
+        encryptionContext := map[keyA := valB];
+      case B =>
+        encryptionContext := map[keyB := valA];
+      case AB =>
+        encryptionContext := map[keyA := valC, keyB := valD];
+      case BA =>
+        encryptionContext := map[keyB := valA, keyA := valB];
+      case C =>
+        encryptionContext := map[keyC := valA];
+      case CE =>
+        encryptionContext := map[keyC := valA, keyD := valB];
+    }
+  }
+
+
+  
+  method NamespaceAndName(n: nat) returns (namespace: string, name: string)
+    requires 0 <= n < 10
+    ensures |namespace| < UINT16_LIMIT
+    ensures |name| < UINT16_LIMIT
+  {
+    var s := "child" + [n as char + '0'];
+    namespace := s + " Namespace";
+    name := s + " Name";
+  }
+  
+  method GenerateKeyPair( keyModulusLength: primitivesTypes.RSAModulusLengthBitsToGenerate )
+    returns (keys: primitivesTypes.GenerateRSAKeyPairOutput)
+  {
+      var crypto :- expect Primitives.AtomicPrimitives();
+
+      keys :- expect crypto.GenerateRSAKeyPair(
+      primitivesTypes.GenerateRSAKeyPairInput(
+          lengthBits := keyModulusLength
+      )
+      );
+  }
+    
 }
