SharedMakefileV2.mk
@@ -73,7 +73,7 @@ verify:
 		-unicodeChar:0 \
 		-functionSyntax:3 \
 		-verificationLogger:csv \
-		-timeLimit:100 \
+		-timeLimit:150 \
 		-trace \
 		`find . -name *.dfy`
 
